finish Types

Coq/Coq30.v
@@ -9,3 +9,214 @@ Add LoadPath "C:\Users\ycy12\Documents\Workspace\LEARNING-STUFF\Coq".
 Load Coq29.
 Hint Constructors multi.
 
+Module Types.
+
+Inductive tm : Type :=
+  | tru : tm
+  | fls : tm
+  | test : tm → tm → tm → tm
+  | zro : tm
+  | scc : tm → tm
+  | prd : tm → tm
+  | iszro : tm → tm.
+
+Inductive bvalue : tm → Prop :=
+  | bv_tru : bvalue tru
+  | bv_fls : bvalue fls.
+Inductive nvalue : tm → Prop :=
+  | nv_zro : nvalue zro
+  | nv_scc : ∀t, nvalue t → nvalue (scc t).
+Definition value (t : tm) := bvalue t ∨ nvalue t.
+Hint Constructors bvalue nvalue.
+Hint Unfold value.
+Hint Unfold t_update.
+
+Reserved Notation "t1 '--->' t2" (at level 40).
+Inductive step : tm → tm → Prop :=
+  | ST_TestTru : ∀t1 t2,
+      (test tru t1 t2) ---> t1
+  | ST_TestFls : ∀t1 t2,
+      (test fls t1 t2) ---> t2
+  | ST_Test : ∀t1 t1' t2 t3,
+      t1 ---> t1' →
+      (test t1 t2 t3) ---> (test t1' t2 t3)
+  | ST_Scc : ∀t1 t1',
+      t1 ---> t1' →
+      (scc t1) ---> (scc t1')
+  | ST_PrdZro :
+      (prd zro) ---> zro
+  | ST_PrdScc : ∀t1,
+      nvalue t1 →
+      (prd (scc t1)) ---> t1
+  | ST_Prd : ∀t1 t1',
+      t1 ---> t1' →
+      (prd t1) ---> (prd t1')
+  | ST_IszroZro :
+      (iszro zro) ---> tru
+  | ST_IszroScc : ∀t1,
+       nvalue t1 →
+      (iszro (scc t1)) ---> fls
+  | ST_Iszro : ∀t1 t1',
+      t1 ---> t1' →
+      (iszro t1) ---> (iszro t1')
+
+where "t1 '--->' t2" := (step t1 t2).
+Hint Constructors step.
+
+Notation step_normal_form := (normal_form step).
+Definition stuck (t : tm) : Prop :=
+  step_normal_form t ∧ ¬value t.
+Hint Unfold stuck.
+
+Example some_term_is_stuck :
+  ∃t, stuck t.
+Proof.
+  exists (scc fls).
+  unfold stuck. split. unfold step_normal_form.
+  intros [t' H]. inversion H;subst. inversion H1.
+  unfold value. intros contra. destruct contra;inversion H;inversion H1.
+Qed.
+
+Lemma value_is_nf : ∀t,
+  value t → step_normal_form t.
+Proof.
+  intros. destruct H;induction H;try (intros [t' H1];inversion H1).
+  apply IHnvalue. exists t1'. auto.
+Qed.
+
+Ltac not_nf x := assert (H' : value x);unfold value;right;auto;apply value_is_nf in H';destruct H';eauto.
+
+Theorem step_deterministic:
+  deterministic step.
+Proof with eauto.
+  unfold deterministic. intros x y1 y2 Hy1 Hy2.
+  generalize dependent y2.
+  induction Hy1; intros y2 Hy2.
+  1 - 2 : inversion Hy2;subst;try reflexivity;inversion H3.
+  inversion Hy2;subst. 1 - 2 : inversion Hy1. apply (IHHy1 t1'0) in H3;subst;auto.
+  inversion Hy2;subst. apply (IHHy1 t1'0) in H0;subst;auto.
+  inversion Hy2;auto. inversion H0.
+  inversion Hy2;subst;auto. inversion H1;subst. assert (value t1).
+  unfold value. right. auto. apply value_is_nf in H0. destruct H0.
+  eauto. inversion Hy2;subst. inversion Hy1. inversion Hy1;subst.
+  assert (value y2).
+  unfold value. right. auto. apply value_is_nf in H. destruct H.
+  eauto. apply (IHHy1 t1'0) in H0;subst;auto.
+  1 - 2 : inversion Hy2;auto;subst;try inversion H0.
+  inversion H1;subst. assert (value t1).
+  unfold value. right. auto. apply value_is_nf in H0. destruct H0.
+  eauto. inversion Hy2;subst. inversion Hy1. inversion Hy1. subst.
+  assert (value t0).
+  unfold value. right. auto. apply value_is_nf in H. destruct H.
+  eauto. apply (IHHy1 t1'0) in H0;subst;auto.
+Qed.
+
+Inductive ty : Type :=
+  | Bool : ty
+  | Nat : ty.
+
+Reserved Notation "'⊢' t '∈' T" (at level 40).
+Inductive has_type : tm → ty → Prop :=
+  | T_Tru :
+       ⊢ tru ∈ Bool
+  | T_Fls :
+       ⊢ fls ∈ Bool
+  | T_Test : ∀t1 t2 t3 T,
+       ⊢ t1 ∈ Bool →
+       ⊢ t2 ∈ T →
+       ⊢ t3 ∈ T →
+       ⊢ test t1 t2 t3 ∈ T
+  | T_Zro :
+       ⊢ zro ∈ Nat
+  | T_Scc : ∀t1,
+       ⊢ t1 ∈ Nat →
+       ⊢ scc t1 ∈ Nat
+  | T_Prd : ∀t1,
+       ⊢ t1 ∈ Nat →
+       ⊢ prd t1 ∈ Nat
+  | T_Iszro : ∀t1,
+       ⊢ t1 ∈ Nat →
+       ⊢ iszro t1 ∈ Bool
+
+where "'⊢' t '∈' T" := (has_type t T).
+Hint Constructors has_type.
+
+Example scc_hastype_nat__hastype_nat : ∀t,
+  ⊢ scc t ∈ Nat →
+  ⊢ t ∈ Nat.
+Proof. inversion 1;auto.
+Qed.
+
+Lemma bool_canonical : ∀t,
+  ⊢ t ∈ Bool → value t → bvalue t.
+Proof.
+  intros t HT [Hb | Hn].
+  - assumption.
+  - induction Hn; inversion HT; auto.
+Qed.
+
+Lemma nat_canonical : ∀t,
+  ⊢ t ∈ Nat → value t → nvalue t.
+Proof.
+  intros t HT [Hb | Hn].
+  - inversion Hb; subst; inversion HT.
+  - assumption.
+Qed.
+
+Theorem progress : ∀t T,
+  ⊢ t ∈ T →
+  value t ∨ ∃t', t ---> t'.
+Proof with auto.
+  intros t T HT.
+  induction HT...
+  - right. inversion IHHT1; clear IHHT1.
+    + apply (bool_canonical t1 HT1) in H.
+      inversion H; subst; clear H.
+      exists t2...
+      exists t3...
+    + inversion H as [t1' H1].
+      exists (test t1' t2 t3)...
+  - inversion IHHT; clear IHHT.
+    + apply (nat_canonical t1 HT) in H. left.
+      inversion H; subst; clear H...
+    + inversion H. right. exists (scc x)...
+  - inversion IHHT; clear IHHT.
+    + apply (nat_canonical t1 HT) in H. right. 
+      inversion H;subst.
+      exists zro... exists t...
+    + inversion H. right. exists (prd x)...
+  - inversion IHHT; clear IHHT.
+    + apply (nat_canonical t1 HT) in H. right.
+      inversion H;subst. exists tru... exists fls...
+    + inversion H. right. exists (iszro x)...
+Qed.
+
+Theorem preservation : ∀t t' T,
+  ⊢ t ∈ T →
+  t ---> t' →
+  ⊢ t' ∈ T.
+Proof with auto.
+  intros t t' T HT HE.
+  generalize dependent t'.
+  induction HT;
+         intros t' HE.
+  1 - 2 : inversion HE.
+  inversion HE; subst; clear HE;try assumption.
+  econstructor; try assumption.
+      apply IHHT1...
+  1 - 3 : inversion HE;subst. inversion HE;subst. econstructor;apply IHHT...
+  auto. eapply scc_hastype_nat__hastype_nat. auto. econstructor...
+  inversion HE;subst;econstructor. apply IHHT...
+Qed.
+
+Definition multistep := (multi step).
+Notation "t1 '-->*' t2" := (multistep t1 t2) (at level 40).
+Corollary soundness : ∀t t' T,
+  ⊢ t ∈ T →
+  t -->* t' →
+  ~(stuck t').
+Proof.
+  intros t t' T HT P. induction P; intros [R S].
+  destruct (progress x T HT); auto.
+  apply IHP. apply (preservation x y T HT H).
+  unfold stuck. split; auto. Qed.
